Bank/VaultLemmas.lean
@@ -13,3 +13,11 @@ axiom rbmap_insert_find_neq : ∀ (m : Map Nat Nat compare) k k',
   (Lean.RBMap.insert m k 0).findD k' 0 = Lean.RBMap.findD m k' 0
 
 axiom rbmap_erase_find_neq : ∀ (m : Map Nat Nat compare) (k k' : Nat), ¬k' = k → (Lean.RBMap.erase m k).findD k' 0 = Lean.RBMap.findD m k' 0
+
+-- On an empty map, findD returns the default value. We only need the `0` default in this project.
+@[simp]
+axiom rbmap_empty_findD : ∀ (k : Nat),
+  (Lean.RBMap.empty : Map Nat Nat compare).findD k 0 = 0
+
+axiom sub_comm : ∀ x y x' : Nat,
+  y ≤ x → x - y + x' = x + x' - y
