BankCorrect.lean
@@ -1,3 +1,22 @@
 import Bank
 
 -- proofs of correctness of the bank
+
+-- WITHDRAW
+
+
+
+-- DEPOSIT
+
+
+
+-- TRANSFER
+-- theorem bank_transfer_transfer_correct : ∀ id qty v_prev v_next,
+
+-- OPEN
+
+
+-- CLOSE
+
+
+-- Balance query
